Proved one path

denotational/Examples.v
@@ -1,10 +1,12 @@
 From ITree Require Import
-     ITree
-     Events.State
-     Events.StateFacts.
+     Basics
+     Subevent
+     Indexed.Sum.
 
 From Coq Require Import
      Fin
+     Lia
+     Vector
      String.
 
 From ExtLib Require Import
@@ -16,33 +18,32 @@ From ExtLib Require Import
      Monads
      Option.
 
-From CTree Require CTrees.
+From Coinduction Require Import
+     coinduction rel tactics.
 
 From CTree Require Import
-     Equ
-     Utils.
+     CTree
+     Interp
+     State
+     Eq
+     SBisim.
 
 From DSL Require Import
      System
      Network
-     Refinement
+     Utils
      Vectors.
 
-Import ITreeNotations.
+From Equations Require Import Equations.
 
-Local Open Scope itree_scope.
+Import MonadNotation.
+Local Open Scope monad_scope.
 Local Open Scope string_scope.
 Local Open Scope vector_scope.
 
 Set Implicit Arguments.
-Set Contextual Implicit.
-
-(** Utility use the standard library *)
-Definition default{T}(o: option T)(d: T): T :=
-  match o with
-  | None => d
-  | Some v => v
-  end.
+Set Strict Implicit.
+Set Asymmetric Patterns.
 
 Module Examples.
   Module Network := Network(DistrSystem).                               
@@ -51,7 +52,7 @@ Module Examples.
   (** Some uids *)
   Program Definition alice : uid 2 := @of_nat_lt 0 2 _.
   Program Definition bob : uid 2 := @of_nat_lt 1 2 _.
-
+  
   (** Some programs *)
   Definition example_alice :=
     a <- load "a";;
@@ -59,30 +60,175 @@ Module Examples.
     a' <- recv;;
     store "b" (payload a').
 
-  Definition example_bob: itree (Storage +' @Net 2) unit :=
+  Definition example_bob: ctree (Storage +' Net 2) unit :=
     m <- recv ;;
     send {| principal := principal m; payload := S (payload m) |}.
 
   (** A Single agent program *)
-  Definition example: itree (Storage +' @Net 1) unit :=
+  Definition example: ctree (Storage +' Net 2) unit :=
     a <- load "a";;
     store "b" (S (default a 0)).
 
+  Definition example_skip: ctree (Storage +' Net 2) unit :=
+    Ret tt.
+
   (** Here we are evaluating two distributed systems to CTrees C1, C2.
       We will show they are equivalent by some sort of Applicative Bisimulation
-      using the leaf equivalence below. *)
+      using the leaf equivalence below. *) 
+ Definition init_heap := (List.cons ("a", 0) List.nil).
 
-  Definition init_heap :=(List.cons ("a", 0) List.nil).
-  Definition C1 := run_network (run_storage [example]) init_heap.
-  Definition C2 := run_network (run_storage [example_alice; example_bob]) init_heap.
+  Definition C1 := run_network (map voidR (run_storage [example; example_skip] init_heap)).
+  Definition C2 := run_network (map voidR (run_storage [example_alice; example_bob] init_heap)).
+
+  Typeclasses eauto := 6.
+
+  Ltac fold_bind :=
+    repeat lazymatch goal with
+           | [ |- sbisim _ (CTree.subst ?k ?t) ] => fold (CTree.bind t k)
+           | [ H: context[CTree.subst ?f ?x] |- _ ] => fold (CTree.bind x f) in H
+           | [ |- context[CTree.subst ?f ?x] ] => fold (CTree.bind x f) in *
+           end.
+
+  Fixpoint fin_all (n : nat) : list (fin n) :=
+    match n as n return list (fin n) with
+    | 0 => List.nil
+    | S n => List.cons (@F1 n) (List.map (@FS _) (fin_all n))
+    end%list.
   
-  Lemma refinement_c1_c2: refinement vec_head_heap_equiv C2 C1.
+  Theorem fin_all_In : forall {n} (f : fin n),
+      List.In f (fin_all n).
   Proof.
-    unfold C2, C1, example, example_alice, example_bob, run_network, run_storage.
-    cbn.
-    (** LOOPS HERE *)
-    setoid_rewrite rewrite_schedule.
+    induction n; intros.
+    inversion f.
+    remember (S n). destruct f.
+    simpl; firstorder.
+    inversion Heqn0. subst.
+    simpl. right. apply List.in_map. auto.
+  Qed.
 
+  Theorem fin_case : forall n (f : fin (S n)),
+      f = F1 \/ exists f', f = FS f'.
+  Proof.
+    intros. generalize (fin_all_In f). intros.
+    destruct H; auto.
+    eapply List.in_map_iff in H. right. destruct H.
+    exists x. intuition.
+  Qed.
+
+  (** Main lemma, C1 is bisimilar to C2 *)
+  Ltac simplify_ds :=
+    repeat lazymatch goal with
+    | [ H: context[schedule_one] |- _] => simp schedule_one in H
+    | [ H: context[get_running] |- _] => simp get_running in H
+    | [ H: context[vector_replace] |- _] => simp vector_replace in H
+    | [ |- context[schedule_one] ] => simp schedule_one
+    | [ |- context[get_running] ] => simp get_running
+    | [ |- context[vector_replace] ] => simp vector_replace
+    end; cbn.
+
+  (** LEF: It folds ~ to `sb bot` must figure out why *)
+  Ltac sb_fwd :=
+    repeat (cbn; lazymatch goal with
+                 | [ |- sbisim (CTree.bind ?t _) (CTree.bind ?t _) ] => apply bind_sbisim_cong
+                 | [ |- sbisim (ChoiceV ?n _) (ChoiceV ?n _) ] => eapply sb_choiceV_id; intros
+                 | [ |- sbisim (ChoiceI ?n _) (ChoiceI ?n _) ] => eapply sb_choiceI_id; intros
+                 | [ |- sbisim (Ret ?x) (Ret ?x) ] => apply reflexivity
+                 | [ |- context[sbisim (TauI _) _] ] => rewrite !sb_tauI
+                 | [ |- context[CTree.bind (Ret _) _] ] => rewrite ?bind_ret_l
+                 | [ |- context[CTree.bind (CTree.bind _ _) _]] => rewrite ?bind_bind
+           end; fold_bind).
+
+  Transparent schedule_one.
+  Transparent schedule_network_0.
+  Transparent get_running.
+  Transparent vector_replace.
+
+
+
+  Lemma sb_c1_c2: C1 ~ C2.
+  Proof.
+    unfold C1, C2, init_heap.
+    (** 
+    setoid_rewrite ctree_eta; sb_fwd. 
+    destruct (fin_case t); intros; subst; simplify_ds.
+    - intro t; destruct (fin_case t); subst; simplify_ds.
+      simp vector_replace.
+      sb_fwd.
+      + simp get_running.
+    *)
+    
+    setoid_rewrite ctree_eta; cbn.
+    
+    eapply sb_choiceI_id; intros; fold_bind; rewrite !bind_ret_l;
+      (** x: fin 2 can be either 1 or 2 *)
+      destruct (fin_case x); subst.
+    
+    - cbn; rewrite !sb_tauI;
+      setoid_rewrite ctree_eta; cbn;
+        eapply sb_choiceI_id; intros; fold_bind; rewrite !bind_ret_l;
+        destruct (fin_case x); subst; cbn.
+      
+      * cbn; rewrite !sb_tauI; 
+        setoid_rewrite ctree_eta; cbn;
+          eapply sb_choiceI_id; intros; fold_bind; rewrite !bind_ret_l;
+          destruct (fin_case x); subst; cbn; rewrite ?bind_ret_l.
+
+        + cbn; rewrite !sb_tauI;
+            setoid_rewrite ctree_eta; cbn;
+            eapply sb_choiceI_id; intros; fold_bind; rewrite !bind_ret_l;
+            destruct (fin_case x); subst; cbn; rewrite ?bind_ret_l.
+          
+          -- cbn; rewrite !sb_tauI;
+               setoid_rewrite ctree_eta; cbn;
+               eapply sb_choiceI_id; intros; fold_bind; rewrite !bind_ret_l;
+               destruct (fin_case x); subst; cbn; rewrite ?bind_ret_l.
+             
+             **  cbn; rewrite !sb_tauI;
+                   setoid_rewrite ctree_eta; cbn; setoid_rewrite bind_ret_l;
+                   fold_bind; cbn; rewrite sb_choiceI1.
+                 
+                 (** Left is DONE -- Choice1 on the right *)
+                 cbn; rewrite sb_tauI; 
+                   setoid_rewrite ctree_eta; cbn;
+                   rewrite sb_choiceI1; cbn; fold_bind; rewrite !bind_ret_l; cbn.
+                 
+                 rewrite !sb_tauI;
+                   setoid_rewrite ctree_eta; cbn;
+                   apply sb_choiceI_r; intros; fold_bind; rewrite ?bind_ret_l;
+                   destruct (fin_case x); subst.
+                 
+                 ++ cbn; rewrite !sb_tauI;
+                      setoid_rewrite ctree_eta; cbn;
+                      apply sb_choiceI_l; intros; fold_bind; rewrite !bind_ret_l;
+                      destruct (fin_case x); subst; cbn; rewrite ?bind_ret_l.
+                    
+                    --- cbn; rewrite !sb_tauI;
+                          setoid_rewrite ctree_eta; cbn;
+                          eapply sb_choiceI_l; intros; fold_bind; rewrite !bind_ret_l;
+                          destruct (fin_case x); subst; cbn; rewrite ?bind_ret_l.
+                        
+                         *** cbn; rewrite !sb_tauI;
+                               setoid_rewrite ctree_eta; cbn;
+                               eapply sb_choiceI_l; intros; fold_bind; rewrite !bind_ret_l;
+                               destruct (fin_case x); subst; cbn; rewrite ?bind_ret_l.
+                             
+                             +++ cbn; rewrite !sb_tauI;
+                                   setoid_rewrite ctree_eta; cbn;
+                                   eapply sb_choiceI_l; intros; fold_bind; rewrite !bind_ret_l;
+                                   destruct (fin_case x); subst; cbn; rewrite ?bind_ret_l.
+                                 
+                                 ---- cbn; rewrite !sb_tauI;
+                                     setoid_rewrite ctree_eta; cbn;
+                                        rewrite sb_choiceI1; intros; fold_bind; rewrite !bind_ret_l; cbn.
+                                      
+                                      rewrite sb_tauI; setoid_rewrite ctree_eta; cbn;
+                                        rewrite sb_choiceI1; intros; fold_bind; rewrite !bind_ret_l; cbn.
+                                      
+                                      rewrite sb_tauI;  setoid_rewrite ctree_eta; cbn.
+                                   (** And finally, the states are equal! *)
+                                   reflexivity.
+           
+  Admitted.
 
 End Examples.
     
