denotational/Network.v
@@ -1,16 +1,12 @@
 From ITree Require Import
-     ITree
-     Events.State.
-
-From CTree Require
-     CTrees.
-
-From Coinduction Require Import
-     coinduction rel tactics.
+     Subevent
+     Indexed.Sum.
 
 From CTree Require Import
-     Equ
-     Utils.
+     CTree
+     Interp.Interp
+     Eq.Equ
+     Core.Utils.
 
 From ExtLib Require Import
      Monad
@@ -18,7 +14,7 @@ From ExtLib Require Import
      RelDec.
 
 From Coq Require Import
-     Vector
+     Vector     
      Fin (* fin definition here *)
      Program.Equality
      Lia.
@@ -28,11 +24,15 @@ From Equations Require Import
 
 From DSL Require Import
      System
+     Utils
      Vectors.
 
-Import CTrees.CTreeNotations.
+From Coinduction Require Import
+     rel coinduction tactics.
 
-Local Open Scope ctree_scope.
+Import EquNotations.
+Import MonadNotation.
+Local Open Scope monad_scope.
 Local Open Scope vector_scope.
 Local Open Scope fin_vector_scope.
 
@@ -45,129 +45,126 @@ Module Network(S: Systems).
   Module Storage := Storage(S).
   Export Monads Storage Messaging S.
 
-  Notation system n R := (vec n (Task n (@Net n) R)).
-
-  Fixpoint num_done{E A m n}(a: vec m (Task n E A)): nat :=
-    match a with
-    | ((Done _ _) :: ts) => S (num_done ts)
-    | ((Running _ _) :: ts) => num_done ts
-    | [] => 0
-    end.
-
-  Fixpoint num_running{E A m n}(a: vec m (Task n E A)): nat :=
-    match a with
-    | ((Done _ _) :: ts) => num_running ts
-    | ((Running _ _) :: ts) => S (num_running ts)
-    | [] => 0
-    end.
-
-  Lemma done_running_inv: forall A E m n (v: vec m (Task n E A)),
-      num_done v + num_running v = m.
-  Proof.
-    intros.
-    dependent induction v.
-    - reflexivity.
-    - destruct h.
-      * cbn; rewrite IHv; reflexivity.
-      * cbn; replace (num_done v + S (num_running v)) with
-          (S (num_done v + num_running v)) by lia;
-          rewrite IHv; reflexivity.
-  Defined.
+  Notation InitSys n E R := (vec n (ctree E R)) (only parsing).
+  Notation Sys n E R := (vec n (Task n E R)) (only parsing).
+  Notation SysLeaf n R := (option (vec n (R * queue n))) (only parsing).
+  Notation SysTree n E R := (ctree E (SysLeaf n R)) (only parsing).
 
   Equations get_running{E A m n}(v: vec m (Task n E A))
-            (i: fin (num_running v)): (fin m * itree E A * queue n) :=
-    get_running ((Running _ _) :: ts) (FS k) := match get_running ts k with
-                                                 | (i, a, q) => (FS i, a, q)
-                                                 end;
-    get_running ((Done a b) :: ts) k := match get_running ts k with
-                                         | (i, a, q) => (FS i, a, q)
-                                         end;
+            (i: fin (num_running v)): (fin m * ctree E A * queue n) :=
+    get_running ((Running _ _) :: ts) (FS k) :=
+      let '(i, a, q) := get_running ts k in (FS i, a, q);
+    get_running ((Done _ _) :: ts) k :=
+      let '(i, a, q) := get_running ts k in (FS i, a, q);
+    get_running ((Blocked _ _) :: ts) k :=
+      let '(i, a, q) := get_running ts k in (FS i, a, q);
     get_running ((Running a q) :: ts) F1 := (F1, a ,q).
-  Transparent get_running.
-  
-  Definition schedule_network_0{E A m n}(a: vec m (Task n E A))
-             {H: num_running a = 0}: vec m (A * queue n).
-    dependent induction a.
-    - exact [].
-    - destruct h; cbn in *.
-      + exact ((r, q) :: IHa H).
-      + inversion H.
-  Defined.
 
-  Equations schedule_network{R: Type}{n: nat}
-             (schedule: system n R ->
-                        CTrees.ctree void1 (vec n (R * queue n)))
-             (sys: system n R):
-    CTrees.ctree void1 (vec n (R * queue n)) :=
-    schedule_network schedule sys :=
-      match num_running sys as n1 return (num_running sys = n1 -> CTrees.ctree void1 (vec n (R * queue n))) with
-      | 0 => fun Hnr: num_running sys = 0 => CTrees.Ret (schedule_network_0 sys)
-      | S n1 =>
-          fun Hnr: num_running sys = S n1 => 
-            (** Non-det pick an agent that is running to execute *)
-            r <- choice true (num_running sys) ;;
-            (** q: the message queue of i *)
-            (** i: The absolute index of a running agent `r`
-                a: The itree of agent `i` (Running)        *)    
-            let '(i, a, q) := get_running sys r in
-            (** Observe the itree `a` *)
-            match observe a with
-            | RetF v =>
-                CTrees.TauI (schedule (sys @ i := Done v q))
-            | TauF t =>
-                CTrees.TauI (schedule (sys @ i := Running t q))
-            | VisF (Send msg) k =>
-                let sys' := sys @ i := Running (k tt) q in
-                let recp := principal msg in
-                match sys' $ recp with
-                | Running a q =>
-                    let msg' := {| principal := i; payload := payload msg |} in
-                    CTrees.TauV (schedule (sys' @ recp := Running a (List.cons msg' q)))
-                | Done _ _ => CTrees.TauV (schedule sys')
-                end
-            (** TODO: Msg delivery non-determinism *)
-            | VisF Recv k =>
-                match last q with 
-                | Some msg =>
-                    (** Pop the msg from the end *)
-                    CTrees.TauV (schedule (sys @ i := Running (k msg) (init q)))
-                | None =>
-                    (** Just loop again if no messages in q *)
-                    CTrees.TauI (schedule sys)
-                end
-            | VisF (Broadcast b) k =>
-                let msg := {| principal := i; payload := b |} in
-                let sys' := map (fun a => match a with
-                                          | Running a q => Running a (List.cons msg q)
-                                          | Done a q => Done a q
-                                          end) sys in 
-                CTrees.TauV (schedule (sys' @ i := Running (k tt) q))
-          (** TODO: NON-det version 
-            sys'' <- mapT (fun a: list Msg * itree Net R =>
-                          let (q', a') := a in
-                          CTrees.choiceV2
-                            (CTrees.Ret (msg :: q', a'))
-                            (CTrees.Ret (q', a'))) sys';;
+  (** Blocking processes might cause a deadlock, in which case we return 'None'
+      or `Some (vec n _)` (every agent returned)
+   *)
+  Equations schedule_network_0 {E A m n} (a: vec m (Task n E A))
+            (H: num_running a = 0): option (vec m (A * queue n)) :=
+    schedule_network_0 [] _ := Some [];
+    schedule_network_0 ((Done r q)::ts) _ :=
+      option_map (fun l => (r, q) :: l) (schedule_network_0 ts _);
+    schedule_network_0 ((Blocked _ _)::ts) _ := None.
+
+  Equations schedule_one{R: Type}{E: Type -> Type}{n: nat}
+            (schedule: Sys n (Net n +' E) R -> SysTree n E R)
+            (sys: Sys n (Net n +' E) R)
+            (r: fin (num_running sys)) : SysTree n E R :=
+    schedule_one schedule sys r with get_running sys r => {
+        schedule_one _ _ _ (i, a, q) with observe a => {
+          (** Returns a value *)
+          schedule_one _ _ _ _ (RetF v) :=
+            TauI (schedule (sys @ i := Done v q));
+        
+          (** A previous choice, traverse it *)
+          schedule_one _ _ _ _ (ChoiceF b n' k) :=
+            Choice b n' (fun i' => schedule (sys @ i := Running (k i') q));
+
+          (** A network `send` effect, interpet it! *)
+          schedule_one _ _ _ _ (VisF (inl1 (Send m)) k) with (sys $ principal m)=>{
+            (** Deliver to running *)
+            schedule_one _ _ _ (i, _, _) _ (Running c q) :=
+              let msg' := {| principal := i; payload := payload m |} in
+              let sys' := sys @ i := Running (k tt) q in
+              let recp := principal m in
+              TauI (schedule (sys' @ recp := Running c (List.cons msg' q)));
             
-            CTrees.TauV (schedule sys'' done)
-          *)
-            end
-      end eq_refl.
+            (** Deliver to blocked processes and unblock them *)
+            schedule_one _ _ _ (i, _, _) _ (Blocked c q) :=
+              let msg' := {| principal := i; payload := payload m |} in
+              let sys' := sys @ i := Running (k tt) q in
+              let recp := principal m in
+              TauI (schedule (sys' @ recp := Running c (List.cons msg' q)));
+            
+            (** Do not deliver to Done processes *)
+            schedule_one _ _ _ (i, _, _) _ (Done _ _) :=
+            TauI (schedule (sys @ i := Running (k tt) q))
+          };
 
-  Transparent schedule_network.
+          (** Receive a message *)
+          schedule_one _ _ _ _ (VisF (inl1 Recv) k) with last q => {
+            (** Pop the msg from the end *)
+            schedule_one _ _ _ (i, _, _) _ (Some msg) :=
+              TauI (schedule (sys @ i := Running (k msg) (init q)));
+            (** Becomes blocked if no messages in q *)
+            schedule_one _ _ _ (i, _, _) _ None :=
+              TauI (schedule (sys @ i := Blocked a q))
+          };
 
-  CoFixpoint schedule {R: Type}{n: nat} := @schedule_network R n schedule.
+          (** Broadcast a message to everyone *)
+          schedule_one _ _ _ _ (VisF (inl1 (Broadcast b)) k) :=
+            let msg := {| principal := i; payload := b |} in
+            let sys' := map (fun a => match a with
+                                      | Running a q => Running a (List.cons msg q)
+                                      | Done a q => Done a q
+                                      | Blocked a q => Running a (List.cons msg q)
+                                      end) sys in 
+            TauI (schedule (sys' @ i := Running (k tt) q));
+              
+          (** Some other downstream effect *)
+          schedule_one _ _ _ _ (VisF (inr1 e) k) :=
+            TauI (schedule (sys @ i := Running (trigger e >>= k) q))
+        }
+      }.
+  (** TODO: NON-det version 
+      sys'' <- mapT (fun a: list Msg * itree Net R =>
+      let (q', a') := a in
+      CTrees.choiceV2
+      (CTrees.Ret (msg :: q', a'))
+      (CTrees.Ret (q', a'))) sys';;
+      
+      CTrees.TauV (schedule sys'' done)
+   *)
 
-  Lemma rewrite_schedule: forall n R (s: system n R), schedule s ≅ schedule_network schedule s.
+  Definition schedule_network{R: Type}{E}{n: nat}
+             (schedule: Sys n (Net n +' E) R -> SysTree n E R)
+             (sys: Sys n (Net n +' E) R): SysTree n E R :=
+    match num_running sys as n1 return
+          (num_running sys = n1 -> SysTree n E R) with
+    | 0 => fun Hnr: num_running sys = 0 =>
+             Ret (schedule_network_0 sys Hnr)
+    | S n1 => fun Hnr: num_running sys = S n1 =>
+                r <- choice false (num_running sys) ;;
+                schedule_one schedule sys r
+    end eq_refl.
+  
+  CoFixpoint schedule {R: Type}{E: Type -> Type}{n: nat} :=
+    @schedule_network R E n schedule.
+
+  Lemma rewrite_schedule: forall n R E (s: Sys n (Net n +' E) R),
+      schedule s ≅ schedule_network schedule s.
   Proof.
-    intros; step; auto.
+    intros.
+    __step_equ.
+    eauto.
   Qed.
 
   (** Evaluates Net *)
-  Definition run_network{R m}(a: stateT heap (fun T => vec m (itree (@Net m) T)) R):
-    stateT heap (fun T => (CTrees.ctree void1 (vec m T))) (R * queue m) :=
-    fun st => (** Need to change the associativity on tuples here, TODO: fix if possible *)
-      CTrees.CTree.map (Vector.map (fun '(h, r, q) => (h, (r, q))))
-                       (schedule (Vector.map (fun it =>
-                                                Running it List.nil) (a st))).
+  Definition run_network{E R n} (s: InitSys n (Net n +' E) R): SysTree n E R :=
+    schedule (Vector.map (fun it => Running it List.nil) s).
+  
 End Network.
