denotational/Vectors.v
@@ -55,17 +55,3 @@ Proof.
         apply andb_true_intro; split; assumption.
 Defined.
 
-
-Fixpoint last{A}(l: list A): option A :=
-  match l with
-  | List.nil => None
-  | List.cons h List.nil => Some h
-  | List.cons h ts => last ts
-  end.
-
-Fixpoint init{A}(l: list A): list A :=
-  match l with
-  | List.nil => List.nil
-  | List.cons h List.nil => List.nil
-  | List.cons h ts => List.cons h (init ts)
-  end.
