denotational/Utils.v
@@ -1,0 +1,57 @@
+(** Random utils *)
+From ITree Require Import
+     Basics
+     Subevent
+     Indexed.Sum
+     Indexed.Function.
+
+From CTree Require Import
+     CTree
+     Interp.
+
+(** Swaps effects *)
+Definition swapES{X Y}: X +' Y ~> Y +' X :=
+  fun _ s => match s with
+             | inr1 x => inl1 x
+             | inl1 y => inr1 y
+             end.
+
+Check elim_void1.
+Definition swap {X Y}: forall T, ctree (X +' Y) T -> ctree (Y +' X) T :=
+  translate (@swapES X Y).
+
+Arguments swap {X Y T}.
+
+Definition voidRES{X}: X ~> X +' void1 := inl1.
+Definition voidLES{X}: X ~> void1 +' X := inr1.
+
+Definition voidR {X}: forall T, ctree X T -> ctree (X +' void1) T :=
+  translate (@voidRES X).
+
+Definition voidL{X}: forall T, ctree X T -> ctree (void1 +' X) T :=
+  translate (@voidLES X).
+
+Arguments voidL {X T}.
+Arguments voidR {X T}.
+
+(** List utils *)
+Fixpoint last{A}(l: list A): option A :=
+  match l with
+  | List.nil => None
+  | List.cons h List.nil => Some h
+  | List.cons h ts => last ts
+  end.
+
+Fixpoint init{A}(l: list A): list A :=
+  match l with
+  | List.nil => List.nil
+  | List.cons h List.nil => List.nil
+  | List.cons h ts => List.cons h (init ts)
+  end.
+
+(** Utility use the standard library *)
+Definition default{T}(o: option T)(d: T): T :=
+  match o with
+  | None => d
+  | Some v => v
+  end.
